vec blake

code/blake2/Hacl.Impl.Blake2.Core.fst
@@ -11,24 +11,8 @@ open Lib.IntVector
 
 module Spec = Spec.Blake2_Vec
 
-type m_spec =
-  | M32
-  | M128
-  | M256
-
 inline_for_extraction
-unfold type word_t (a:Spec.alg) = Spec.word_t a
-
-inline_for_extraction
-unfold let element_t (a:Spec.alg) (m:m_spec) =
-  match a,m with
-  | Spec.Blake2S,M128 -> (vec_t U32 4)
-  | Spec.Blake2S,M256 -> (vec_t U32 4)
-  | Spec.Blake2B,M256 -> (vec_t U64 4)
-  | _ -> (word_t a)
-
-inline_for_extraction
-unfold let zero_element (a:Spec.alg) (m:m_spec) : element_t a m =
+let zero_element (a:Spec.alg) (m:m_spec) : element_t a m =
   match a,m with
   | Spec.Blake2S,M128 -> (vec_zero U32 4)
   | Spec.Blake2S,M256 -> (vec_zero U32 4)
@@ -36,19 +20,13 @@ unfold let zero_element (a:Spec.alg) (m:m_spec) : element_t a m =
   | _ -> Spec.zero a
 
 inline_for_extraction
-unfold let row_len (a:Spec.alg) (m:m_spec) : size_t =
+let row_len (a:Spec.alg) (m:m_spec) : size_t =
   match a,m with
   | Spec.Blake2S,M128 -> 1ul
   | Spec.Blake2S,M256 -> 1ul
   | Spec.Blake2B,M256 -> 1ul
   | _ -> 4ul
 
-inline_for_extraction
-unfold let row_p (a:Spec.alg) (m:m_spec) =
-  lbuffer (element_t a m) (row_len a m)
-
-inline_for_extraction
-val row_v: #a:Spec.alg -> #m:m_spec -> h:mem -> row_p a m -> GTot (Spec.row a)
 inline_for_extraction
 let row_v #a #m h r =
   match a,m with
@@ -57,28 +35,9 @@ let row_v #a #m h r =
   | Spec.Blake2B,M256 -> vec_v (Lib.Sequence.index (as_seq h r) 0)
   | _ -> as_seq h r
 
-noextract
-val row_v_lemma: #a:Spec.alg -> #m:m_spec -> h0:mem -> h1:mem -> r:row_p a m ->
-  Lemma (ensures (as_seq h0 r == as_seq h1 r ==>
-		  row_v h0 r == row_v h1 r))
-	[SMTPat (row_v h0 r); SMTPat (row_v h1 r)]
 let row_v_lemma #a #m h0 h1 r = ()
 
-inline_for_extraction
-unfold let state_p (a:Spec.alg) (m:m_spec) =
-  lbuffer (element_t a m) (4ul *. row_len a m)
-
-inline_for_extraction
-unfold let index_t = n:size_t{v n < 4}
-
-inline_for_extraction
-let g_rowi (#a:Spec.alg) (#m:m_spec) (st:state_p a m)  (idx:index_t) : GTot (row_p a m) =
-  gsub st (idx *. row_len a m) (row_len a m)
-
-#push-options "--z3rlimit  50"
-val g_rowi_disjoint: #a:Spec.alg -> #m:m_spec -> st:state_p a m -> idx1:index_t -> idx2:index_t ->
-  Lemma (ensures (idx1 <> idx2 ==> disjoint (g_rowi st idx1) (g_rowi st idx2)))
-	[SMTPat (disjoint (g_rowi st idx1) (g_rowi st idx2))]
+#push-options "--z3rlimit 50"
 let g_rowi_disjoint #a #m st idx1 idx2 =
   if idx1 <. idx2 then (
     assert (v (idx1 *. row_len a m) + v (row_len a m) <= v (idx2 *. row_len a m));
@@ -95,10 +54,6 @@ let g_rowi_disjoint #a #m st idx1 idx2 =
     LowStar.Monotonic.Buffer.loc_disjoint_gsub_buffer #_ #((LowStar.Buffer.trivial_preorder (element_t a m))) #((LowStar.Buffer.trivial_preorder (element_t a m))) st (idx1 *. row_len a m) (row_len a m) (LowStar.Buffer.trivial_preorder (element_t a m)) (idx2 *. row_len a m) (row_len a m) (LowStar.Buffer.trivial_preorder (element_t a m)))
   else ()
 
-val g_rowi_unchanged: #a:Spec.alg -> #m:m_spec -> h0:mem -> h1:mem -> st:state_p a m -> i:index_t ->
-  Lemma (requires (as_seq h0 st == as_seq h1 st))
-	(ensures (as_seq h0 (g_rowi st i) == as_seq h1 (g_rowi st i)))
-	[SMTPat (as_seq h0 (g_rowi st i)); SMTPat (as_seq h1 (g_rowi st i))]
 let g_rowi_unchanged #a #m h0 h1 st i =
   assert (v (i *. row_len a m) + v (row_len a m) <= length st);
   LowStar.Monotonic.Buffer.as_seq_gsub #_ #(LowStar.Buffer.trivial_preorder (element_t a m)) #(LowStar.Buffer.trivial_preorder (element_t a m)) h0 st (i *. row_len a m) (row_len a m)
@@ -106,16 +61,13 @@ let g_rowi_unchanged #a #m h0 h1 st i =
   LowStar.Monotonic.Buffer.as_seq_gsub #_ #(LowStar.Buffer.trivial_preorder (element_t a m)) #(LowStar.Buffer.trivial_preorder (element_t a m)) h1 st (i *. row_len a m) (row_len a m)
   (LowStar.Buffer.trivial_preorder (element_t a m))
 
-val g_rowi_disjoint_other:  #a:Spec.alg -> #m:m_spec -> #b:Type -> #len:size_t -> st:state_p a m -> i:index_t -> x:lbuffer b len ->
-  Lemma(requires (disjoint st x))
-       (ensures (disjoint (g_rowi st i) x /\ disjoint x (g_rowi st i)))
 let g_rowi_disjoint_other #a #m #b #len st i x =
   assert (v (i *. row_len a m) + v (row_len a m) <= length st);
     LowStar.Monotonic.Buffer.loc_includes_gsub_buffer_r'  #_ #(LowStar.Buffer.trivial_preorder (element_t a m)) #(LowStar.Buffer.trivial_preorder (element_t a m)) st (i *. row_len a m) (row_len a m)
   (LowStar.Buffer.trivial_preorder (element_t a m))
 #pop-options
 
-inline_for_extraction
+inline_for_extraction noextract
 let state_v (#a:Spec.alg) (#m:m_spec) (h:mem) (st:state_p a m) : GTot (Spec.state a) =
   let r0 = row_v h (g_rowi st 0ul) in
   let r1 = row_v h (g_rowi st 1ul) in
@@ -123,19 +75,10 @@ let state_v (#a:Spec.alg) (#m:m_spec) (h:mem) (st:state_p a m) : GTot (Spec.stat
   let r3 = row_v h (g_rowi st 3ul) in
   create4 r0 r1 r2 r3
 
-noextract
-val state_v_lemma: #a:Spec.alg -> #m:m_spec -> h0:mem -> h1:mem -> st:state_p a m ->
-  Lemma (requires (as_seq h0 st == as_seq h1 st))
-	(ensures (state_v h0 st == state_v h1 st))
-	[SMTPat (state_v h0 st); SMTPat (state_v h1 st)]
 let state_v_lemma #a #m h0 h1 st = ()
 
 
 #push-options "--z3rlimit 50"
-val modifies_row: a:Spec.alg -> m:m_spec -> h0:mem -> h1:mem -> st:state_p a m -> i:index_t ->
-  Lemma (requires (live h0 st /\ modifies (loc (g_rowi st i)) h0 h1))
-	(ensures (state_v h1 st == Lib.Sequence.((state_v h0 st).[v i] <- row_v h1 (g_rowi st i))))
-	[SMTPat (modifies (loc (g_rowi st i)) h0 h1)]
 let modifies_row a m h0 h1 st i =
     assert (live h0 (g_rowi st 0ul));
     assert (live h0 (g_rowi st 1ul));
@@ -146,22 +89,10 @@ let modifies_row a m h0 h1 st i =
 
 
 inline_for_extraction
-val rowi: #a:Spec.alg -> #m:m_spec -> st:state_p a m -> idx:index_t ->
-	  ST (row_p a m)
-	  (requires (fun h -> live h st))
-	  (ensures (fun h0 r h1 -> h0 == h1 /\ live h1 r /\ r == g_rowi st idx))
-
-inline_for_extraction
 let rowi (#a:Spec.alg) (#m:m_spec) (st:state_p a m)  (idx:index_t) =
   sub st (idx *. row_len a m) (row_len a m)
 
 
-inline_for_extraction
-val xor_row: #a:Spec.alg -> #m:m_spec -> r1:row_p a m -> r2:row_p a m ->
-	  ST unit
-	  (requires (fun h -> live h r1 /\ live h r2 /\ disjoint r1 r2))
-	  (ensures (fun h0 _ h1 -> modifies (loc r1) h0 h1 /\
-				row_v h1 r1 == Spec.( row_v h0 r1 ^| row_v h0 r2 )))
 inline_for_extraction
 let xor_row #a #m r1 r2 =
   match a,m with
@@ -175,12 +106,6 @@ let xor_row #a #m r1 r2 =
 
 
 inline_for_extraction
-val add_row: #a:Spec.alg -> #m:m_spec -> r1:row_p a m -> r2:row_p a m ->
-	  ST unit
-	  (requires (fun h -> live h r1 /\ live h r2 /\ disjoint r1 r2))
-	  (ensures (fun h0 _ h1 -> modifies (loc r1) h0 h1 /\
-				row_v h1 r1 == Spec.( row_v h0 r1 +| row_v h0 r2 )))
-inline_for_extraction
 let add_row #a #m r1 r2 =
   match a,m with
   | Spec.Blake2S,M128 ->
@@ -192,12 +117,6 @@ let add_row #a #m r1 r2 =
   | _ -> map2T 4ul r1 (add_mod #(Spec.wt a) #SEC) r1 r2
 
 
-inline_for_extraction
-val ror_row: #a:Spec.alg -> #m:m_spec -> r1:row_p a m -> r2:rotval (Spec.wt a) ->
-	  ST unit
-	  (requires (fun h -> live h r1))
-	  (ensures (fun h0 _ h1 -> modifies (loc r1) h0 h1 /\
-				row_v h1 r1 == Spec.( row_v h0 r1 >>>| r2 )))
 inline_for_extraction
 let ror_row #a #m r1 r2 =
   match a,m with
@@ -211,13 +130,6 @@ let ror_row #a #m r1 r2 =
     let r1:lbuffer (Spec.word_t a) 4ul = r1 in
     mapT 4ul r1 (rotate_right_i #(Spec.wt a) #SEC r2) r1
 
-
-inline_for_extraction
-val permr_row: #a:Spec.alg -> #m:m_spec -> r1:row_p a m -> n:index_t ->
-	  ST unit
-	  (requires (fun h -> live h r1))
-	  (ensures (fun h0 _ h1 -> modifies (loc r1) h0 h1 /\
-				row_v h1 r1 == Spec.( rotr (row_v h0 r1) (v n) )))
 
 #push-options "--z3rlimit 50"
 inline_for_extraction
@@ -256,9 +168,6 @@ let permr_row #a #m r1 n =
 #pop-options
 
 #push-options "--z3rlimit 50"
-val create4_lemma: #a:Type -> x0:a -> x1:a -> x2:a -> x3:a ->
-  Lemma (ensures (Lib.Sequence.createL [x0;x1;x2;x3] == create4 x0 x1 x2 x3))
-	[SMTPat (Lib.Sequence.createL [x0;x1;x2;x3])]
 let create4_lemma #a x0 x1 x2 x3 =
   let open Lib.Sequence in
   let l : list a = [x0;x1;x2;x3] in
@@ -272,23 +181,8 @@ let create4_lemma #a x0 x1 x2 x3 =
 #pop-options
 
 inline_for_extraction
-val alloc_row: a:Spec.alg -> m:m_spec ->
-	  StackInline (row_p a m)
-	  (requires (fun h -> True))
-	  (ensures (fun h0 r h1 -> stack_allocated r h0 h1 (Lib.Sequence.create (v (row_len a m)) (zero_element a m)) /\
-				live h1 r /\
-				row_v h1 r == Spec.zero_row a))
-
-inline_for_extraction
 let alloc_row a m = create (row_len a m) (zero_element a m)
 
-
-inline_for_extraction
-val create_row: #a:Spec.alg -> #m:m_spec -> r1:row_p a m -> w0:word_t a -> w1:word_t a -> w2:word_t a -> w3:word_t a ->
-	  ST unit
-	  (requires (fun h -> live h r1))
-	  (ensures (fun h0 _ h1 -> modifies (loc r1) h0 h1 /\
-				row_v h1 r1 == Spec.( create_row w0 w1 w2 w3 )))
 
 inline_for_extraction
 let create_row #a #m r w0 w1 w2 w3 =
@@ -306,22 +200,7 @@ let create_row #a #m r w0 w1 w2 w3 =
     Lib.Sequence.eq_intro (as_seq h1 r) (create4 w0 w1 w2 w3)
 
 inline_for_extraction
-val load_row: #a:Spec.alg -> #m:m_spec -> r1:row_p a m -> ws:lbuffer (word_t a) 4ul ->
-	  ST unit
-	  (requires (fun h -> live h r1 /\ live h ws /\ disjoint r1 ws))
-	  (ensures (fun h0 _ h1 -> modifies (loc r1) h0 h1 /\
-				row_v h1 r1 == Spec.( load_row (as_seq h0 ws))))
-
-inline_for_extraction
 let load_row #a #m r ws = create_row r ws.(0ul) ws.(1ul) ws.(2ul) ws.(3ul)
-
-inline_for_extraction
-val gather_row: #a:Spec.alg -> #ms:m_spec -> #len:size_t -> r:row_p a ms -> m:lbuffer uint8 len ->
-          i0: Spec.word_index a (v len) -> i1:Spec.word_index a (v len) -> i2:Spec.word_index a (v len) -> i3:Spec.word_index a (v len)
-	  -> ST unit
-	  (requires (fun h -> live h r /\ live h m /\ disjoint r m))
-	  (ensures (fun h0 _ h1 -> modifies (loc r) h0 h1 /\
-				row_v h1 r == Spec.( gather_row (as_seq h0 m) i0 i1 i2 i3)))
 
 #push-options "--z3rlimit 100"
 inline_for_extraction
