code/blake2/Hacl.Impl.Blake2.Core.fsti
@@ -1,0 +1,155 @@
+module Hacl.Impl.Blake2.Core
+module ST = FStar.HyperStack.ST
+open FStar.HyperStack
+open FStar.HyperStack.All
+open FStar.Mul
+
+open Lib.IntTypes
+open Lib.Buffer
+open Lib.ByteBuffer
+open Lib.IntVector
+
+module Spec = Spec.Blake2_Vec
+
+type m_spec =
+  | M32
+  | M128
+  | M256
+
+inline_for_extraction
+unfold type word_t (a:Spec.alg) = Spec.word_t a
+
+inline_for_extraction
+unfold let element_t (a:Spec.alg) (m:m_spec) =
+  match a,m with
+  | Spec.Blake2S,M128 -> (vec_t U32 4)
+  | Spec.Blake2S,M256 -> (vec_t U32 4)
+  | Spec.Blake2B,M256 -> (vec_t U64 4)
+  | _ -> (word_t a)
+
+inline_for_extraction
+val zero_element: a:Spec.alg -> m:m_spec -> element_t a m
+
+inline_for_extraction
+val row_len: a:Spec.alg -> m:m_spec -> size_t
+
+
+inline_for_extraction
+unfold let row_p (a:Spec.alg) (m:m_spec) =
+  lbuffer (element_t a m) (row_len a m)
+
+inline_for_extraction
+val row_v: #a:Spec.alg -> #m:m_spec -> h:mem -> row_p a m -> GTot (Spec.row a)
+
+noextract
+val row_v_lemma: #a:Spec.alg -> #m:m_spec -> h0:mem -> h1:mem -> r:row_p a m ->
+  Lemma (ensures (as_seq h0 r == as_seq h1 r ==>
+		  row_v h0 r == row_v h1 r))
+	[SMTPat (row_v h0 r); SMTPat (row_v h1 r)]
+
+inline_for_extraction
+unfold let state_p (a:Spec.alg) (m:m_spec) =
+  lbuffer (element_t a m) (4ul *. row_len a m)
+
+inline_for_extraction
+unfold let index_t = n:size_t{v n < 4}
+
+inline_for_extraction
+let g_rowi (#a:Spec.alg) (#m:m_spec) (st:state_p a m)  (idx:index_t) : GTot (row_p a m) =
+  gsub st (idx *. row_len a m) (row_len a m)
+
+val g_rowi_disjoint: #a:Spec.alg -> #m:m_spec -> st:state_p a m -> idx1:index_t -> idx2:index_t ->
+  Lemma (ensures (idx1 <> idx2 ==> disjoint (g_rowi st idx1) (g_rowi st idx2)))
+	[SMTPat (disjoint (g_rowi st idx1) (g_rowi st idx2))]
+
+val g_rowi_unchanged: #a:Spec.alg -> #m:m_spec -> h0:mem -> h1:mem -> st:state_p a m -> i:index_t ->
+  Lemma (requires (as_seq h0 st == as_seq h1 st))
+	(ensures (as_seq h0 (g_rowi st i) == as_seq h1 (g_rowi st i)))
+	[SMTPat (as_seq h0 (g_rowi st i)); SMTPat (as_seq h1 (g_rowi st i))]
+
+val g_rowi_disjoint_other:  #a:Spec.alg -> #m:m_spec -> #b:Type -> #len:size_t -> st:state_p a m -> i:index_t -> x:lbuffer b len ->
+  Lemma(requires (disjoint st x))
+       (ensures (disjoint (g_rowi st i) x /\ disjoint x (g_rowi st i)))
+
+
+inline_for_extraction noextract
+val state_v: #a:Spec.alg -> #m:m_spec -> mem -> state_p a m -> GTot (Spec.state a)
+
+noextract
+val state_v_lemma: #a:Spec.alg -> #m:m_spec -> h0:mem -> h1:mem -> st:state_p a m ->
+  Lemma (requires (as_seq h0 st == as_seq h1 st))
+	(ensures (state_v h0 st == state_v h1 st))
+	[SMTPat (state_v h0 st); SMTPat (state_v h1 st)]
+
+
+val modifies_row: a:Spec.alg -> m:m_spec -> h0:mem -> h1:mem -> st:state_p a m -> i:index_t ->
+  Lemma (requires (live h0 st /\ modifies (loc (g_rowi st i)) h0 h1))
+	(ensures (state_v h1 st == Lib.Sequence.((state_v h0 st).[v i] <- row_v h1 (g_rowi st i))))
+	[SMTPat (modifies (loc (g_rowi st i)) h0 h1)]
+
+
+inline_for_extraction
+val rowi: #a:Spec.alg -> #m:m_spec -> st:state_p a m -> idx:index_t ->
+	  ST (row_p a m)
+	  (requires (fun h -> live h st))
+	  (ensures (fun h0 r h1 -> h0 == h1 /\ live h1 r /\ r == g_rowi st idx))
+
+inline_for_extraction
+val xor_row: #a:Spec.alg -> #m:m_spec -> r1:row_p a m -> r2:row_p a m ->
+	  ST unit
+	  (requires (fun h -> live h r1 /\ live h r2 /\ disjoint r1 r2))
+	  (ensures (fun h0 _ h1 -> modifies (loc r1) h0 h1 /\
+				row_v h1 r1 == Spec.( row_v h0 r1 ^| row_v h0 r2 )))
+inline_for_extraction
+val add_row: #a:Spec.alg -> #m:m_spec -> r1:row_p a m -> r2:row_p a m ->
+	  ST unit
+	  (requires (fun h -> live h r1 /\ live h r2 /\ disjoint r1 r2))
+	  (ensures (fun h0 _ h1 -> modifies (loc r1) h0 h1 /\
+				row_v h1 r1 == Spec.( row_v h0 r1 +| row_v h0 r2 )))
+inline_for_extraction
+val ror_row: #a:Spec.alg -> #m:m_spec -> r1:row_p a m -> r2:rotval (Spec.wt a) ->
+	  ST unit
+	  (requires (fun h -> live h r1))
+	  (ensures (fun h0 _ h1 -> modifies (loc r1) h0 h1 /\
+				row_v h1 r1 == Spec.( row_v h0 r1 >>>| r2 )))
+inline_for_extraction
+val permr_row: #a:Spec.alg -> #m:m_spec -> r1:row_p a m -> n:index_t ->
+	  ST unit
+	  (requires (fun h -> live h r1))
+	  (ensures (fun h0 _ h1 -> modifies (loc r1) h0 h1 /\
+				row_v h1 r1 == Spec.( rotr (row_v h0 r1) (v n) )))
+
+val create4_lemma: #a:Type -> x0:a -> x1:a -> x2:a -> x3:a ->
+  Lemma (ensures (Lib.Sequence.createL [x0;x1;x2;x3] == create4 x0 x1 x2 x3))
+	[SMTPat (Lib.Sequence.createL [x0;x1;x2;x3])]
+
+inline_for_extraction
+val alloc_row: a:Spec.alg -> m:m_spec ->
+	  StackInline (row_p a m)
+	  (requires (fun h -> True))
+	  (ensures (fun h0 r h1 -> stack_allocated r h0 h1 (Lib.Sequence.create (v (row_len a m)) (zero_element a m)) /\
+				live h1 r /\
+				row_v h1 r == Spec.zero_row a))
+
+inline_for_extraction
+val create_row: #a:Spec.alg -> #m:m_spec -> r1:row_p a m -> w0:word_t a -> w1:word_t a -> w2:word_t a -> w3:word_t a ->
+	  ST unit
+	  (requires (fun h -> live h r1))
+	  (ensures (fun h0 _ h1 -> modifies (loc r1) h0 h1 /\
+				row_v h1 r1 == Spec.( create_row w0 w1 w2 w3 )))
+inline_for_extraction
+val load_row: #a:Spec.alg -> #m:m_spec -> r1:row_p a m -> ws:lbuffer (word_t a) 4ul ->
+	  ST unit
+	  (requires (fun h -> live h r1 /\ live h ws /\ disjoint r1 ws))
+	  (ensures (fun h0 _ h1 -> modifies (loc r1) h0 h1 /\
+				row_v h1 r1 == Spec.( load_row (as_seq h0 ws))))
+
+inline_for_extraction
+val gather_row: #a:Spec.alg -> #ms:m_spec -> #len:size_t -> r:row_p a ms -> m:lbuffer uint8 len ->
+          i0: Spec.word_index a (v len) -> i1:Spec.word_index a (v len) -> i2:Spec.word_index a (v len) -> i3:Spec.word_index a (v len)
+	  -> ST unit
+	  (requires (fun h -> live h r /\ live h m /\ disjoint r m))
+	  (ensures (fun h0 _ h1 -> modifies (loc r) h0 h1 /\
+				row_v h1 r == Spec.( gather_row (as_seq h0 m) i0 i1 i2 i3)))
+
+
